Semantic type for own.

types.v
@@ -2,13 +2,14 @@ From iris.program_logic Require Import thread_local.
 From lrust Require Export notation.
 From lrust Require Import lifetime heap.
 
+Definition mgmtE := nclose tlN ∪ lftN.
+
 Section defs.
 
   Context `{heapG Σ, lifetimeG Σ, thread_localG Σ}.
 
   Record type :=
-    { ty_size : nat;
-      ty_dup : bool;
+    { ty_size : nat; ty_dup : bool;
       ty_own : thread_id → list val → iProp Σ;
       ty_shr : lifetime → thread_id → coPset → loc → iProp Σ;
 
@@ -16,14 +17,17 @@ Section defs.
 
       ty_size_eq tid vl : ty_own tid vl ⊢ length vl = ty_size;
       ty_dup_dup tid vl : ty_dup → ty_own tid vl ⊢ ty_own tid vl ★ ty_own tid vl;
-      ty_shr_share E N κ l tid q : N ⊥ tlN → N ⊥ lftN →
-        nclose N ⊆ E → nclose tlN ⊆ E → nclose lftN ⊆ E →
+      (* The mask for starting the sharing does /not/ include the
+         namespace N, because sharing can be triggered in a context
+         where N is open. This should not be harmful, since sharing
+         typically creates invariants, which does not need the mask. *)
+      ty_share E N κ l tid q : nclose N ⊥ mgmtE → mgmtE ⊆ E →
         lft κ ⊢ &{κ} (l ↦★: ty_own tid) ★ [κ]{q}
                 ={E}=> ty_shr κ tid N l ★ [κ]{q};
       ty_shr_mono κ κ' tid E E' l : E ⊆ E' →
         κ' ⊑ κ ⊢ ty_shr κ tid E l → ty_shr κ' tid E' l;
       ty_shr_acc κ tid E E' l q :
-        E ⊆ E' → nclose lftN ⊆ E' → nclose tlN ⊆ E' → ty_dup →
+        E ⊆ E' → mgmtE ⊆ E' → ty_dup →
         ty_shr κ tid E l ⊢
           [κ]{q} ★ tl_own tid E ={E'}=> ∃ q', ▷l ↦★{q'}: ty_own tid ★
              (▷l ↦★{q'}: ty_own tid ={E'}=★ [κ]{q} ★ tl_own tid E)
@@ -36,32 +40,30 @@ Section defs.
      (□ ∀ κ tid E l, ty1.(ty_shr) κ tid E l → ty2.(ty_shr) κ tid E l))%I.
 
   Record simple_type :=
-    { st_size : nat;
-      st_dup : bool;
+    { st_size : nat; st_dup : bool;
       st_own : thread_id → list val → iProp Σ;
 
       st_size_eq tid vl : st_own tid vl ⊢ length vl = st_size;
       st_dup_dup tid vl : st_dup → st_own tid vl ⊢ st_own tid vl ★ st_own tid vl
     }.
 
-  Program Coercion ty_of_st (st : simple_type) : type :=
-    {| ty_size := st.(st_size);
-       ty_dup := st.(st_dup);
+  Program Definition ty_of_st (st : simple_type) : type :=
+    {| ty_size := st.(st_size); ty_dup := st.(st_dup);
        ty_own := st.(st_own);
        ty_shr := λ κ tid _ l, (&frac{κ} λ q, l ↦★{q}: st.(st_own) tid)%I
     |}.
   Next Obligation. apply st_size_eq. Qed.
   Next Obligation. apply st_dup_dup. Qed.
   Next Obligation.
-    intros st E N κ l tid q ?????. iIntros "#Hκ !# [Hmt Hlft]".
+    intros st E N κ l tid q ??. iIntros "#Hκ !# [Hmt Hlft]".
     iVs (lft_borrow_fracture with "[Hmt]"); last by iFrame. done.
   Qed.
   Next Obligation.
     iIntros (st κ κ' tid E E' l _) "#Hord". by iApply lft_frac_borrow_incl.
   Qed.
   Next Obligation.
-    intros st κ tid E E' l q ????.  iIntros "#Hshr!#[Hlft Htlown]".
-    iVs (lft_frac_borrow_open with "[] Hlft"); first done; last by iFrame.
+    intros st κ tid E E' l q ???.  iIntros "#Hshr!#[Hlft Htlown]".
+    iVs (lft_frac_borrow_open with "[] Hlft"); first set_solver; last by iFrame.
     iSplit; last done. iIntros "!#". iIntros (q1 q2). iSplit; iIntros "H".
     - iDestruct "H" as (vl) "[Hq1q2 Hown]".
       iDestruct (st_dup_dup with "Hown") as "[Hown1 Hown2]". done.
@@ -81,47 +83,100 @@ End defs.
 
 Module Types.
 Section types.
+  (* TODO : make ty_of_st work as a coercion. *)
 
   Context `{heapG Σ, lifetimeG Σ, thread_localG Σ}.
 
-  (* FIXME : why does not the coercion work ?  *)
   Program Definition bot : type :=
-    ty_of_st {| st_size := 1;
-       st_dup := true;
+    ty_of_st {| st_size := 1; st_dup := true;
        st_own tid vl := False%I
     |}.
   Next Obligation. iIntros (tid vl) "[]". Qed.
   Next Obligation. iIntros (tid vl _) "[]". Qed.
 
-  (* FIXME : idem *)
   Program Definition unit : type :=
-    ty_of_st {| st_size := 0;
-       st_dup := true;
+    ty_of_st {| st_size := 0;  st_dup := true;
        st_own tid vl := (vl = [])%I
     |}.
   Next Obligation. iIntros (tid vl) "%". by subst. Qed.
   Next Obligation. iIntros (tid vl _) "%". auto. Qed.
 
-  (* FIXME : idem  *)
   Program Definition bool : type :=
-    ty_of_st {| st_size := 1;
-       st_dup := true;
-       st_own tid vl := (∃ z:bool, vl = [ #z ]%V)%I
+    ty_of_st {| st_size := 1; st_dup := true;
+       st_own tid vl := (∃ z:bool, vl = [ #z ])%I
     |}.
   Next Obligation. iIntros (tid vl) "H". iDestruct "H" as (z) "%". by subst. Qed.
   Next Obligation. iIntros (tid vl _) "H". auto. Qed.
 
-  (* FIXME : idem  *)
   Program Definition int : type :=
-    ty_of_st {| st_size := 1;
-       st_dup := true;
-       st_own tid vl := (∃ z:Z, vl = [ #z ]%V)%I
+    ty_of_st {| st_size := 1; st_dup := true;
+       st_own tid vl := (∃ z:Z, vl = [ #z ])%I
     |}.
   Next Obligation. iIntros (tid vl) "H". iDestruct "H" as (z) "%". by subst. Qed.
   Next Obligation. iIntros (tid vl _) "H". auto. Qed.
 
-  
-
+  Program Definition own (q:Qp) (ty:type) :=
+    {| ty_size := 1; ty_dup := false;
+       ty_own tid vl :=
+         (∃ l:loc, vl = [ #l ] ★ †{q}l…ty.(ty_size)
+                                 ★ ▷ l ↦★: ty.(ty_own) tid)%I;
+       ty_shr κ tid E l :=
+         (∃ l':loc, &frac{κ}(λ q', l ↦{q'} #l') ★
+            ∀ q', □ ([κ]{q'} →|={E ∪ mgmtE, mgmtE}▷=> ty.(ty_shr) κ tid E l' ★ [κ]{q'}))%I
+    |}.
+  Next Obligation.
+    iIntros (q ty tid vl) "H". iDestruct "H" as (l) "[% _]". by subst.
+  Qed.
+  Next Obligation. intros _ _ _ _ []. Qed.
+  Next Obligation.
+    intros q ty E N κ l tid q' ?? =>/=.
+    iIntros "#Hκ!#[Hshr Hq']".
+    iVs (lft_borrow_open with "[Hshr Hq']") as "[Hown Hob]". set_solver. by iFrame.
+    iDestruct "Hown" as (vl) "[Hmt Hvl]". iDestruct "Hvl" as (l') "(>%&Hf&Hown)".
+    subst.
+    iVs (lft_open_borrow_contravar with "[Hob Hf]") as "Hob". set_solver.
+    { iSplitR "Hob"; last done. iIntros "!>[Hmt1 Hmt2]!==>!>". iExists [ #l' ].
+      rewrite heap_mapsto_vec_singleton. iSplitL "Hmt1"; first done.
+      iExists _. iSplit; [|by iSplitR "Hmt2"]. done. }
+    iVs (lft_borrow_close with "[Hmt Hown Hob]") as "[Hb Htok]". set_solver.
+    { rewrite heap_mapsto_vec_singleton. iSplitR "Hob"; last done.
+      by iIntros "!>{$Hmt$Hown}". }
+    iVs (lft_borrow_split with "Hb") as "[Hb1 Hb2]". set_solver.
+    iVs (lft_borrow_fracture _ _ (λ q, l ↦{q} #l')%I with "Hb1") as "Hbf".
+    rewrite lft_borrow_persist.
+    iDestruct "Hb2" as (κ' i) "(#Hord&#Hpb&Hpbown)".
+    iVs (inv_alloc N _ (lft_pers_borrow_own i κ' ∨ ty_shr ty κ tid N l')%I
+         with "[Hpbown]") as "#Hinv"; first by eauto.
+    iIntros "!==>{$Htok}". iExists l'. iFrame.
+    iIntros (q'') "!#Htok". iVs (inv_open with "Hinv") as "[[>Hbtok|#Hshr] Hclose]".
+      set_solver.
+    - replace ((nclose N ∪ mgmtE) ∖ N) with mgmtE by set_solver.
+      iAssert (&{κ}▷ l' ↦★: ty_own ty tid)%I with "[Hbtok]" as "Hb".
+      { rewrite lft_borrow_persist. eauto. }
+      iVs (lft_borrow_open with "[Hb Htok]") as "[Hown Hob]". set_solver. by iFrame.
+      iVs (lft_open_borrow_contravar with "[Hob]") as "Hob". set_solver.
+      { iSplitR "Hob"; last done. instantiate (1:=(l' ↦★: ty_own ty tid)%I). eauto 10. }
+      iIntros "!==>!>".
+      iVs (lft_borrow_close with "[Hown Hob]") as "[Hb Htok]". set_solver.
+        by iFrame "Hown".
+      iVs (ty.(ty_share) with "Hκ [Hb Htok]") as "[#Hshr Htok]"; try done. by iFrame.
+      iVs ("Hclose" with "[]") as "_"; by eauto.
+    - replace ((nclose N ∪ mgmtE) ∖ N) with mgmtE by set_solver.
+      iIntros "!==>!>". iVs ("Hclose" with "[]") as "_"; by eauto.
+  Qed.
+  Next Obligation.
+    intros _ ty κ κ' tid E E' l ?. iIntros "#Hκ #H".
+    iDestruct "H" as (l') "[Hfb Hvs]". iExists l'.
+    iSplit. by iApply (lft_frac_borrow_incl with "[]").
+    iIntros (q') "!#Htok".
+    iVs (lft_incl_trade with "Hκ Htok") as (q'') "[Htok Hclose]". set_solver.
+    iApply (pvs_trans _ (E ∪ mgmtE)). iApply pvs_intro'. set_solver.
+    iIntros "Hclose'". iVs ("Hvs" $! q'' with "Htok") as "Hvs'".
+    iIntros "!==>!>". iVs "Hvs'" as "[Hshr Htok]". iVs "Hclose'".
+    iVs ("Hclose" with "Htok"). iFrame.
+    iApply (ty.(ty_shr_mono) with "Hκ"); last done. done.
+  Qed.
+  Next Obligation. done. Qed.
 
 End types.
 
